Verif_bst.v
@@ -7,446 +7,11 @@ Require Import bst.
 Instance CompSpecs : compspecs. make_compspecs prog. Defined.
 Definition Vprog : varspecs.  mk_varspecs prog. Defined.
 
-(* Required for `dependent induction` tactic *)
 Require Import Coq.Program.Equality.
 
-(* Some custom tactics *)
 Require Import my_tactics.
-
-(* BST specification *)
-
-Inductive bin_tree (A: Type) : Type := 
-  | leaf : bin_tree A
-  | node : A -> bin_tree A -> bin_tree A -> bin_tree A.
-Arguments bin_tree _%type_scope.
-Arguments leaf {A}%type_scope.
-Arguments node {A}%type_scope.
-
-(* bin_tree with *exactly* one hole *)
-Inductive bin_tree_hole (A: Type) : Type :=
-  | hole : bin_tree_hole A
-  | node_hole_l : A -> bin_tree_hole A -> bin_tree A -> bin_tree_hole A
-  | node_hole_r : A -> bin_tree A -> bin_tree_hole A -> bin_tree_hole A.
-Arguments bin_tree_hole _%type_scope.
-Arguments hole {A}%type_scope.
-Arguments node_hole_l {A}%type_scope.
-Arguments node_hole_r {A}%type_scope.
-
-Fixpoint fill_hole {A} (outer: bin_tree_hole A) (inner: bin_tree A) : bin_tree A :=
-  match outer with 
-  | hole => inner
-  | node_hole_l a l r => node a (fill_hole l inner) r
-  | node_hole_r a l r => node a l (fill_hole r inner)
-  end.
-
-Fixpoint extend_hole {A} (outer inner: bin_tree_hole A) : bin_tree_hole A :=
-  match outer with 
-  | hole => inner
-  | node_hole_l a l r => node_hole_l a (extend_hole l inner) r
-  | node_hole_r a l r => node_hole_r a l (extend_hole r inner)
-  end.
-
-Inductive bin_tree_forall {A} : bin_tree A -> (A -> Prop) -> Prop :=
-  | bin_tree_forall_leaf : forall p, bin_tree_forall leaf p 
-  | bin_tree_forall_node : forall (p: A -> Prop) a l r,
-      p a -> bin_tree_forall l p -> bin_tree_forall r p -> bin_tree_forall (node a l r) p.
-
-Inductive well_ordered {A} : bin_tree (Z * A) -> Prop :=
-  | well_ordered_leaf : well_ordered leaf 
-  | well_ordered_node : forall k v l r,
-      bin_tree_forall l (fun n => fst n < k) -> 
-      bin_tree_forall r (fun n => fst n > k) -> 
-      well_ordered l ->
-      well_ordered r ->
-      well_ordered (node (k, v) l r).
-
-Definition bst A := bin_tree (Z * A).
-Definition bst_hole A := bin_tree_hole (Z * A).
-
-Inductive is_subtree {A} : bin_tree A -> bin_tree A -> Prop :=
-  | is_subtree_refl  : forall b, is_subtree b b 
-  | is_subtree_left  : forall b n l r, is_subtree b l -> is_subtree b (node n l r)
-  | is_subtree_right : forall b n l r, is_subtree b r -> is_subtree b (node n l r).
-
-Lemma is_subtree_leaf : forall {A} (b: bin_tree A), is_subtree leaf b.
-Proof.
-  intros A b.
-  induction b; constructor; assumption.
-Qed.
-
-Theorem subtree_forall : forall {A} sub b (p: A -> Prop),
-  is_subtree sub b -> bin_tree_forall b p -> bin_tree_forall sub p.
-Proof.
-  intros.
-  induction H;
-  try (apply IHis_subtree; inversion H0);
-  assumption.
-Qed.
-
-Theorem subtree_well_ordered : forall {A} (b sub: bst A),
-  is_subtree sub b -> well_ordered b -> well_ordered sub.
-Proof.
-  intros.
-  induction b.
-  - destruct sub.
-    + constructor.
-    + inversion H.
-  - inversion H; subst.
-    + assumption.
-    + inversion H0; apply IHb1; assumption.
-    + inversion H0; apply IHb2; assumption.
-Qed.
-
-Fixpoint insert {A} (k: Z) (v: A) (b: bst A) : bst A :=
-  match b with 
-  | leaf => node (k, v) leaf leaf
-  | node (k', v') l r => 
-      match k ?= k' with 
-      | Eq => node (k', v) l r 
-      | Lt => node (k', v') (insert k v l) r 
-      | Gt => node (k', v') l (insert k v r)
-      end 
-  end.
-
-Lemma insert_forall {A} : forall (p: (Z * A) -> Prop) k v bst,
-  p (k, v) -> bin_tree_forall bst p -> bin_tree_forall (insert k v bst) p.
-Proof.
-  intros p k v b H.
-  induction b; intro H0; simpl.
-  - constructor; assumption.
-  - destruct_pair. find_Z_compare_destruct;
-    inversion H0; subst; constructor; 
-    try (apply IHb1 + apply IHb2); 
-    assumption.
-Qed.
-
-Theorem insert_well_ordered {A}: forall (b: bst A) k v, 
-  well_ordered b -> well_ordered (insert k v b).
-Proof.
-  intro b; induction b; intros k v H; simpl.
-  - repeat constructor.
-  - inversion H; subst.
-    find_Z_compare_destruct;
-    constructor; try (apply insert_forall + apply IHb1 + apply IHb2); assumption.
-Qed.
-
-Fixpoint pop_min {A} (a: Z * A) (l r: bst A) : (Z * A) * bst A :=
-  match l with
-  | leaf => (a, r)
-  | node a' l' r' =>
-      let (min_a, popped_l) := pop_min a' l' r'
-      in (min_a, node a popped_l r)
-  end.
-
-Lemma pop_min_forall_1 {A} : forall (p: (Z * A) -> Prop) a l r,
-  bin_tree_forall (node a l r) p -> p (fst (pop_min a l r)).
-Proof.
-  intros p a l; revert p a.
-  induction l; intros; simpl.
-  - inversion H; assumption.
-  - destruct (pop_min a l1 l2) eqn:H_pop.
-    simpl.
-    replace p0 with (fst (pop_min a l1 l2)) by (rewrite H_pop; reflexivity).
-    apply IHl1.
-    inversion H; assumption.
-Qed.
-
-Lemma pop_min_forall_2 {A} : forall (p: (Z * A) -> Prop) a l r,
-  bin_tree_forall (node a l r) p -> bin_tree_forall (snd (pop_min a l r)) p.
-Proof.
-  intros p a l; revert p a.
-  induction l; intros; simpl.
-  - inversion H; assumption.
-  - destruct (pop_min a l1 l2) eqn:H_pop.
-    simpl.
-    replace b with (snd (pop_min a l1 l2)) by (rewrite H_pop; reflexivity).
-    constructor.
-    + inversion H; assumption.
-    + apply IHl1. inversion H; assumption.
-    + inversion H; assumption.
-Qed.
-
-Theorem bin_tree_forall_strengthen {A} : forall (p q: (Z * A) -> Prop) b,
-  (forall x, p x -> q x) -> bin_tree_forall b p -> bin_tree_forall b q.
-Proof.
-  intros.
-  dependent induction H0; subst; constructor; simplify_assumps.
-  - apply H. assumption.
-  - assumption.
-  - assumption.
-Qed.
-
-Lemma pop_min_is_min {A} : forall (a: Z * A) l r,
-  well_ordered (node a l r) ->
-  bin_tree_forall (snd (pop_min a l r)) (fun n => fst n > fst (fst (pop_min a l r))).
-Proof.
-  intros a l; revert a.
-  induction l; intros; simpl.
-  - inversion H; assumption.
-  - destruct (pop_min a l1 l2) eqn:H_pop.
-    replace p with (fst (pop_min a l1 l2)) by (rewrite H_pop; reflexivity).
-    replace b with (snd (pop_min a l1 l2)) by (rewrite H_pop; reflexivity).
-    simpl.
-    constructor.
-    + inversion H; subst.
-      simpl.
-      apply pop_min_forall_1 in H3.
-      lia.
-    + apply IHl1. inversion H; assumption.
-    + inversion H; subst.
-      eapply bin_tree_forall_strengthen; [|eassumption].
-      intros [x].
-      simpl.
-      enough (k > fst (fst (pop_min a l1 l2))); [lia|].
-      apply pop_min_forall_1 in H3.
-      lia.
-Qed.
-
-Theorem pop_min_well_ordered {A} : forall (a: Z * A) l r,
-  well_ordered (node a l r) -> well_ordered (snd (pop_min a l r)).
-Proof.
-  intros a l; revert a.
-  induction l; intros; simpl.
-  - inversion H; assumption.
-  - destruct (pop_min a l1 l2) eqn:H_pop.
-    simpl.
-    replace b with (snd (pop_min a l1 l2)) by (rewrite H_pop; reflexivity).
-    destruct a0; constructor.
-    + apply pop_min_forall_2. inversion H; assumption.
-    + inversion H; assumption.
-    + apply IHl1. inversion H; assumption.
-    + inversion H; assumption.
-Qed.
-
-Fixpoint delete {A} (k: Z) (b: bst A) : bst A := 
-  match b with 
-  | leaf => leaf
-  | node (k', v) l r => 
-      match k ?= k' with 
-      | Eq => match l with
-          | leaf => r
-          | _ => match r with 
-              | leaf => leaf
-              | node ra rl rr =>
-                  let (min_a, popped_r) := pop_min ra rl rr
-                  in node min_a l popped_r
-              end
-          end
-      | Lt => delete k l
-      | Gt => delete k r
-      end 
-  end.
-
-Lemma delete_forall {A} : forall (p: (Z * A) -> Prop) k bst,
-  bin_tree_forall bst p -> bin_tree_forall (delete k bst) p.
-Proof.
-  intros p k b.
-  induction b as [|[k' v] l IH1 r IH2]; intro H; simpl; [assumption|].
-  find_Z_compare_destruct.
-  - destruct l, r; try (inversion H; assumption).
-    destruct (pop_min p1 r1 r2) eqn:H_pop.
-    constructor.
-    + replace p2 with (fst (pop_min p1 r1 r2)) by (rewrite H_pop; reflexivity).
-      apply pop_min_forall_1.
-      inversion H; assumption.
-    + inversion H; assumption.
-    + replace b with (snd (pop_min p1 r1 r2)) by (rewrite H_pop; reflexivity).
-      apply pop_min_forall_2.
-      inversion H; assumption.
-  - apply IH1. inversion H; assumption.
-  - apply IH2. inversion H; assumption.
-Qed.
-
-
-Theorem delete_well_ordered {A}: forall (b: bst A) k, 
-  well_ordered b -> well_ordered (delete k b).
-Proof.
-  intros b; induction b as [|[k' v] l IH1 r IH2]; intros k H; simpl; [constructor|].
-  find_Z_compare_destruct.
-  - destruct l, r; try (inversion H; assumption).
-    destruct (pop_min p0 r1 r2) eqn:H_pop.
-    destruct_pair.
-    constructor.
-    + inversion H; subst.
-      eapply bin_tree_forall_strengthen; [|eassumption].
-      intros [x].
-      simpl.
-      enough (k' < z); [lia|].
-      apply pop_min_forall_1 in H5.
-      rewrite H_pop in H5.
-      simpl in H5.
-      lia.
-    + replace b with (snd (pop_min p0 r1 r2)) by (rewrite H_pop; reflexivity).
-      replace z with (fst (fst (pop_min p0 r1 r2))) by (rewrite H_pop; reflexivity).
-      apply pop_min_is_min.
-      inversion H; assumption.
-    + inversion H; assumption.
-    + replace b with (snd (pop_min p0 r1 r2)) by (rewrite H_pop; reflexivity).
-      apply pop_min_well_ordered.
-      inversion H; assumption.
-  - apply IH1. inversion H; assumption.
-  - apply IH2. inversion H; assumption.
-Qed.
-
-Fixpoint search {A} (k: Z) (b: bst A) : bst A := 
-  match b with 
-  | leaf => leaf
-  | node (k', v) l r => 
-      match k ?= k' with 
-      | Eq => b
-      | Lt => search k l
-      | Gt => search k r
-      end 
-  end.
-
-Lemma wo_node_eq {A} : forall k (v1 v2: A) l1 l2 r1 r2,
-  well_ordered (node (k,v1) l1 r1) ->
-  is_subtree (node (k,v2) l2 r2) (node (k,v1) l1 r1) ->
-  node (k,v1) l1 r1 = node (k,v2) l2 r2.
-Proof.
-  intros.
-  inversion H0; subst.
-  - reflexivity. 
-  - inversion H; subst. 
-    eapply subtree_forall in H3; [|eassumption].
-    inversion H3; subst.
-    simpl in H5. lia.
-  - inversion H; subst. 
-    eapply subtree_forall in H3; [|eassumption].
-    inversion H3; subst.
-    simpl in H5. lia.
-Qed.
-
-Lemma wo_subtree_left {A} : forall k1 k2 (v1 v2: A) l1 l2 r1 r2,
-  well_ordered (node (k1,v1) l1 r1) ->
-  is_subtree (node (k2,v2) l2 r2) (node (k1,v1) l1 r1) ->
-  k2 < k1 ->
-  is_subtree (node (k2,v2) l2 r2) l1.
-Proof.
-  intros.
-  inversion H0; subst.
-  - lia.
-  - assumption.
-  - inversion H; subst.
-    eapply subtree_forall in H4; [|eassumption].
-    inversion H4; subst.
-    simpl in H6. lia.
-Qed.
-
-Lemma wo_subtree_right {A} : forall k1 k2 (v1 v2: A) l1 l2 r1 r2,
-  well_ordered (node (k1,v1) l1 r1) ->
-  is_subtree (node (k2,v2) l2 r2) (node (k1,v1) l1 r1) ->
-  k2 > k1 ->
-  is_subtree (node (k2,v2) l2 r2) r1.
-Proof.
-  intros.
-  inversion H0; subst.
-  - lia.
-  - inversion H; subst.
-    eapply subtree_forall in H4; [|eassumption].
-    inversion H4; subst.
-    simpl in H6. lia.
-  - assumption.
-Qed.
-
-Theorem search_spec {A} : forall (b: bst A) k v l r,
-  well_ordered b ->
-  is_subtree (node (k,v) l r) b ->
-  search k b = node (k,v) l r.
-Proof.
-  intros.
-  induction b.
-  - inversion H0.
-  - inversion H; subst.
-    simplify_assumps.
-    simpl.
-    find_Z_compare_destruct.
-    + eapply wo_node_eq; assumption.
-    + apply IHb1.
-      eapply wo_subtree_left; eassumption.
-    + apply IHb2.
-      eapply wo_subtree_right; eassumption.
-Qed.
-
-(* This acts as a complement to search - where search returns the subtree, this returns the original tree,
-   but with a hole where the subtree used to be. *)
-Fixpoint search_make_hole {A} (k: Z) (b: bst A) : bst_hole A := 
-  match b with 
-  | leaf => hole
-  | node (k', v) l r => 
-      match k ?= k' with 
-      | Eq => hole
-      | Lt => node_hole_l (k', v) (search_make_hole k l) r
-      | Gt => node_hole_r (k', v) l (search_make_hole k r)
-      end 
-  end.
-
-Theorem fill_search_hole {A} : forall k (b: bst A),
-  fill_hole (search_make_hole k b) (search k b) = b.
-Proof.
-  intros k b.
-  induction b.
-  - reflexivity.
-  - simpl.
-    destruct_pair.
-    find_Z_compare_destruct; simpl.
-    + reflexivity.
-    + f_equal. assumption.
-    + f_equal. assumption.
-Qed.
-
-(* This does search and search_make_hole together *)
-Fixpoint split_bst_at {A} (k: Z) (b: bst A) : bst_hole A * bst A :=
-  match b with 
-  | leaf => (hole, leaf)
-  | node (k', v) l r =>
-      match k ?= k' with 
-      | Eq => (hole, b)
-      | Lt => let (outer, inner) := split_bst_at k l 
-              in (node_hole_l (k', v) outer r, inner)
-      | Gt => let (outer, inner) := split_bst_at k r 
-              in (node_hole_r (k', v) l outer, inner)
-      end 
-  end.
-
-Theorem search_is_subtree : forall {A} k (b sub: bst A),
-  search k b = sub -> is_subtree sub b.
-Proof.
-  intros A k b sub.
-  induction b; try destruct_pair; simpl; intro H.
-  - subst. constructor.
-  - find_Z_compare_destruct.
-    + constructor.
-    + apply is_subtree_left.
-      apply IHb1.
-      assumption.
-    + apply is_subtree_right.
-      apply IHb2.
-      assumption.
-Qed.
-
-Lemma search_well_ordered : forall {A} k (b sub: bst A),
-  search k b = sub -> well_ordered b -> well_ordered sub.
-Proof.
-  intros.
-  eapply subtree_well_ordered.
-  eapply search_is_subtree.
-  eassumption.
-  assumption.
-Qed.
-
-Theorem search_insert {A}: forall k v (b: bst A),
-  exists l r, search k (insert k v b) = node (k, v) l r.
-Proof.
-  intros k v b.
-  induction b.
-  - simpl.
-    rewrite Z.compare_refl.
-    unify_goal.
-  - simpl. destruct_pair.
-    find_Z_compare_destruct;
-    simpl; rewrite Heqc; assumption + unify_goal.
-Qed.
+Require Import bst_spec.
+Require Import bst_holes.
 
 (* BST representations *)
 
@@ -494,9 +59,39 @@ Fixpoint bst_hole_rep (b: bst_hole Z) (p: val): mpred :=
         bst_hole_rep r pr
   end.
 
-(* Definition bst_rep_w_ptr b head k sub := 
-  let (outer, inner) := split_bst_at k b
-  in (bst_hole_rep outer head * bst_rep inner sub)%logic. *)
+Definition ptr_to_bst_rep b p := EX q, data_at Ews (tptr t_bst) q p * bst_rep b q.
+
+Theorem generalize_ptr_to_node_rep : forall b p q,
+  data_at Ews (tptr t_bst) q p * bst_rep b q |-- ptr_to_bst_rep b p.
+Proof.
+  intros.
+  unfold ptr_to_bst_rep.
+  EExists.
+  entailer!.
+Qed.
+
+Fixpoint ptr_to_bst_hole_rep b p := 
+  match b with 
+  | hole => emp
+  | node_hole_l (k,v) l r =>
+      EX (q pr: val),
+        data_at Ews (tptr t_bst) q p *
+        malloc_token Ews t_bst q *
+        field_at Ews t_bst [StructField _key] (Vint (Int.repr k)) q *
+        field_at Ews t_bst [StructField _val] (Vint (Int.repr v)) q *
+        field_at Ews t_bst [StructField _right] pr q *
+        ptr_to_bst_hole_rep l (field_address t_bst [StructField _left] q) *
+        bst_rep r pr
+  | node_hole_r (k,v) l r =>
+      EX (q pl: val),
+        data_at Ews (tptr t_bst) q p *
+        malloc_token Ews t_bst q *
+        field_at Ews t_bst [StructField _key] (Vint (Int.repr k)) q *
+        field_at Ews t_bst [StructField _val] (Vint (Int.repr v)) q *
+        field_at Ews t_bst [StructField _left] pl q *
+        bst_rep l pl *
+        ptr_to_bst_hole_rep r (field_address t_bst [StructField _right] q)
+  end.
 
 Lemma bst_rep_local_prop: forall b p,
   bst_rep b p |-- !! (is_pointer_or_null p /\ (p = nullval <-> b = leaf)).
@@ -523,7 +118,8 @@ Hint Resolve bst_rep_valid_pointer : valid_pointer.
 
 (* Function specifications *) 
 
-Definition new_bst_spec: ident * funspec := DECLARE _new_bst
+Definition new_bst_spec: ident * funspec :=
+  DECLARE _new_bst
   WITH k: Z, v: Z, gv: globals
   PRE [tint, tint]
     PROP (repable_signed k; repable_signed v)
@@ -534,6 +130,21 @@ Definition new_bst_spec: ident * funspec := DECLARE _new_bst
       PROP ()
       RETURN (p)
       SEP (bst_rep (node (k, v) leaf leaf) p; mem_mgr gv).
+
+Definition search_bst_spec: ident * funspec := 
+  DECLARE _search_bst 
+  WITH head: val, k: Z, b: bst Z, gv: globals 
+  PRE [tptr t_bst, tint]
+    PROP (repable_signed k;
+          bin_tree_forall b (fun n => repable_signed (fst n));
+          well_ordered b)
+    PARAMS (head; Vint (Int.repr k)) GLOBALS (gv)
+    SEP (bst_rep b head; mem_mgr gv)
+  POST [tptr t_bst] 
+    EX vret,
+      PROP ()
+      RETURN (vret)
+      SEP (bst_hole_rep (search_make_hole k b) head; bst_rep (search k b) vret; mem_mgr gv).
 
 Definition insert_bst_spec: ident * funspec :=
   DECLARE _insert_bst
@@ -554,26 +165,31 @@ Definition insert_bst_spec: ident * funspec :=
            bst_rep (insert k v b) new_bst;
            mem_mgr gv).
 
-Definition search_bst_spec: ident * funspec := 
-  DECLARE _search_bst 
-  WITH head: val, k: Z, b: bst Z, gv: globals 
-  PRE [tptr t_bst, tint]
-    PROP (repable_signed k;
-          bin_tree_forall b (fun n => repable_signed (fst n));
-          well_ordered b)
-    PARAMS (head; Vint (Int.repr k)) GLOBALS (gv)
-    SEP (bst_rep b head; mem_mgr gv)
-  POST [tptr t_bst] 
-    EX vret,
+Definition pop_min_spec: ident * funspec :=
+  DECLARE _pop_min
+  WITH bst_ptr: val, head: val, a: (Z * Z), l: bst Z, r: bst Z, gv: globals
+  PRE [tptr (tptr t_bst)]
+    PROP (bin_tree_forall (node a l r) (fun n => repable_signed (fst n));
+          well_ordered (node a l r))
+    PARAMS (bst_ptr) GLOBALS (gv)
+    SEP (data_at Ews (tptr t_bst) head bst_ptr;
+         bst_rep (node a l r) head;
+         mem_mgr gv)
+  POST [tptr t_bst]
+    EX min: val, EX new_bst: val, EX r': bst Z,
       PROP ()
-      RETURN (vret)
-      SEP (bst_hole_rep (search_make_hole k b) head; bst_rep (search k b) vret; mem_mgr gv).
+      RETURN (min)
+      SEP (data_at Ews (tptr t_bst) new_bst bst_ptr; 
+           bst_rep (rm_min a l r) new_bst;
+           (* Does this need to be a hole instead? *)
+           bst_rep (node (get_min a l r) leaf r') min;
+           mem_mgr gv).
 
 Definition delete_bst_spec: ident * funspec :=
   DECLARE _delete_bst
   WITH parent_ptr: val, parent: val, k: Z, b: bst Z, gv: globals
   PRE [tptr (tptr t_bst), tint]
-    PROP (repable_signed k; repable_signed v;
+    PROP (repable_signed k;
           bin_tree_forall b (fun n => repable_signed (fst n));
           well_ordered b)
     PARAMS (parent_ptr; Vint (Int.repr k)) GLOBALS (gv)
@@ -589,297 +205,10 @@ Definition delete_bst_spec: ident * funspec :=
            mem_mgr gv).
 
 Definition Gprog: funspecs := 
-  ltac:(with_library prog [new_bst_spec; insert_bst_spec; search_bst_spec]).
+  ltac:(with_library prog [new_bst_spec; search_bst_spec; insert_bst_spec; pop_min_spec; delete_bst_spec]).
 
 (* Proofs of C functions *)
 
-(* But first, some definitions for the invariants *)
-
-(* The direction of transitivity here is nice for induction, but doesn't correspond 
-   to the intuitive direction in which a path grows. *)
-Inductive search_path : Z -> bst Z -> bst Z -> Prop := 
-  | path_refl : forall k b, search_path k b b
-  | path_step_l : forall k k' v l r b,
-      search_path k l b -> k < k' -> search_path k (node (k',v) l r) b
-  | path_step_r : forall k k' v l r b,
-      search_path k r b -> k > k' -> search_path k (node (k',v) l r) b.
-
-(* Definition search_path_rep (k: Z) (outer inner: bst Z) : mpred :=
-  !! (search_path k outer inner) && () *)
-
-(* This is the direction a path will actually grow in *)
-Lemma path_step_down_l : forall k head k' v l r,
-  search_path k head (node (k',v) l r) -> k < k' -> search_path k head l.
-Proof.
-  intros. dependent induction H.
-  - apply path_step_l.
-    + constructor. 
-    + assumption.
-  - apply path_step_l.
-    + eapply IHsearch_path; trivial.
-    + assumption. 
-  - apply path_step_r.
-    + eapply IHsearch_path; trivial.
-    + assumption.
-Qed.
-Lemma path_step_down_r : forall k head k' v l r,
-  search_path k head (node (k',v) l r) -> k > k' -> search_path k head r.
-Proof.
-  intros. dependent induction H.
-  - apply path_step_r.
-    + constructor. 
-    + assumption.
-  - apply path_step_l.
-    + eapply IHsearch_path; trivial.
-    + assumption. 
-  - apply path_step_r.
-    + eapply IHsearch_path; trivial.
-    + assumption.
-Qed.
-
-Theorem search_path_fail : forall k b, search_path k b leaf -> search k b = leaf.
-Proof.
-  intros. dependent induction H.
-  - reflexivity.
-  - simpl.
-    rewrite Zaux.Zcompare_Lt by assumption.
-    apply IHsearch_path.
-    reflexivity.
-  - simpl.
-    rewrite Zaux.Zcompare_Gt by lia.
-    apply IHsearch_path.
-    reflexivity.
-Qed.
-
-(* Theorem search_path_fail_hole : forall k b,
-  search_path k b leaf -> search_make_hole k b = b.
-Proof.
-  intros k b H.
-  induction b.
-  - reflexivity.
-  - simpl.
-    destruct_pair.
-    find_Z_compare_destruct.
-    + find_contradiction.
-    + f_equal.
-      apply IHb1.
-      inversion H; subst.
-      * assumption.
-      * lia.
-    + f_equal.
-      apply IHb2.
-      inversion H; subst.
-      * lia.
-      * assumption.
-Qed.
- *)
-
-Theorem search_path_success: forall k b v l r,
-  search_path k b (node (k,v) l r) -> search k b = (node (k,v) l r).
-Proof.
-  intros. dependent induction H.
-  - simpl.
-    rewrite Z.compare_refl.
-    reflexivity.
-  - simpl.
-    rewrite Zaux.Zcompare_Lt by assumption. 
-    apply IHsearch_path.
-    reflexivity.
-  - simpl.
-    rewrite Zaux.Zcompare_Gt by lia.
-    apply IHsearch_path.
-    reflexivity.
-Qed.
-
-Lemma search_path_constant : forall k b1 b2,
-  search_path k b1 b2 -> search k b1 = search k b2.
-Proof.
-  intros k b1 b2 H.
-  dependent induction H; simpl.
-  - reflexivity.
-  - rewrite Zaux.Zcompare_Lt; assumption.
-  - rewrite Zaux.Zcompare_Gt by lia. assumption.
-Qed.
-
-Theorem search_path_is_subtree: forall k b sub, search_path k b sub -> is_subtree sub b.
-Proof.
-  intros.
-  induction H.
-  - constructor.
-  - apply is_subtree_left. assumption.
-  - apply is_subtree_right. assumption.
-Qed.
-
-Definition proper_subtree {A} (b1 b2: bin_tree A) := b1 <> b2 /\ is_subtree b1 b2.
-
-Ltac break_let :=
-  match goal with
-    | [ H : context [ (let (_,_) := ?X in _) ] |- _ ] => destruct X eqn:?
-    | [ |- context [ (let (_,_) := ?X in _) ] ] => destruct X eqn:?
-  end.
-
-(* Intended for when `search_path k outer inner` *)
-Definition bst_subtract_path k (outer inner: bst Z) : bst_hole Z :=
-  match inner with 
-  | leaf => search_make_hole k outer
-  | node (k',v) l r => search_make_hole k' outer 
-  end.
-
-Lemma bst_subtract_path_b_b : forall k b, bst_subtract_path k b b = hole.
-Proof.
-  intros.
-  destruct b.
-  - reflexivity.
-  - simpl.
-    break_let.
-    rewrite Z.compare_refl.
-    reflexivity.
-Qed.
-
-Theorem fill_hole_bst_subtract_path: forall k b sub,
-  well_ordered b ->
-  search_path k b sub ->
-  fill_hole (bst_subtract_path k b sub) sub = b.
-Proof.
-  intros k b sub H_wo H_path.
-  induction H_path.
-  - destruct b.
-    + reflexivity.
-    + simpl.
-      destruct_pair.
-      rewrite Z.compare_refl.
-      reflexivity.
-  - inversion H_wo; subst.
-    simplify_assumps.
-    destruct b.
-    + simpl.
-      rewrite Zaux.Zcompare_Lt by assumption.
-      simpl.
-      f_equal.
-      simpl in *.
-      assumption.
-    + simpl.
-      destruct_pair.
-      simpl in *.
-      apply search_path_is_subtree in H_path.
-      find_Z_compare_destruct.
-      * eapply subtree_forall in H_path; [|eassumption].
-        inversion H_path; subst.
-        simpl in *.
-        lia.
-      * simpl.
-        f_equal.
-        assumption.
-      * eapply subtree_forall in H_path; [|eapply H4].
-        inversion H_path; subst.
-        simpl in *.
-        lia.
-  - inversion H_wo; subst.
-    simplify_assumps.
-    destruct b.
-    + simpl.
-      rewrite Zaux.Zcompare_Gt by lia.
-      simpl.
-      f_equal.
-      simpl in *.
-      assumption.
-    + simpl.
-      destruct_pair.
-      simpl in *.
-      apply search_path_is_subtree in H_path.
-      find_Z_compare_destruct.
-      * eapply subtree_forall in H_path; [|eassumption].
-        inversion H_path; subst.
-        simpl in *.
-        lia.
-      * eapply subtree_forall in H_path; [|eapply H5].
-        inversion H_path; subst.
-        simpl in *.
-        lia.
-      * simpl.
-        f_equal.
-        assumption.
-Qed.
-
-Theorem is_subtree_up_left {A}: forall (a: A) l r b,
-  is_subtree (node a l r) b -> is_subtree l b.
-Proof.
-  intros.
-  dependent induction H.
-  - apply is_subtree_left. constructor.
-  - apply is_subtree_left.
-    eapply IHis_subtree.
-    reflexivity.
-  - apply is_subtree_right.
-    eapply IHis_subtree.
-    reflexivity.
-Qed.
-
-Theorem is_subtree_up_right {A}: forall (a: A) l r b,
-  is_subtree (node a l r) b -> is_subtree r b.
-Proof.
-  intros.
-  dependent induction H.
-  - apply is_subtree_right. constructor.
-  - apply is_subtree_left.
-    eapply IHis_subtree.
-    reflexivity.
-  - apply is_subtree_right.
-    eapply IHis_subtree.
-    reflexivity.
-Qed.
-
-(* Alternatively, base this on a "proper" search_path *)
-(* Theorem hole_rep_fuse_left2 : forall search_k k v l r k' v' l' r' (curr head pl pr: val),
-  well_ordered (node (k,v) l r) ->
-  search_path search_k (node (k,v) l r) (node (k',v') l' r') ->
-  search_k < k' ->
-  (node (k,v) l r = node (k',v') l' r' -> head = curr) ->
-    bst_hole_rep (bst_subtract_path k (node (k,v) l r) (node (k',v') l' r')) head *
-    malloc_token Ews t_bst curr *
-    data_at Ews t_bst (Vint (Int.repr k'), (Vint (Int.repr v'), (pl, pr))) curr *
-    bst_rep r' pr
-    |-- bst_hole_rep (bst_subtract_path search_k (node (k,v) l r) l') head.
-Proof.
-  intros search_k k v l r.
-  induction (node (k,v) l r).
-  - intros. inversion H0.
-  -
-    intros.
-    simpl.
-    destruct_pair.
-    find_Z_compare_destruct.
-    + apply search_path_is_subtree in H0.
-      apply wo_node_eq in H0; [|assumption].
-      inversion H0; subst.
-      simplify_assumps; subst.
-      simpl; cancel.
-      destruct l'.
-      * simpl.
-        rewrite Zaux.Zcompare_Lt by assumption.
-        simpl.
-        repeat EExists.
-        entailer!.
-      * simpl. 
-        destruct_pair.
-        rewrite Z.compare_refl.
-        rewrite Zaux.Zcompare_Lt.
-        -- simpl.
-           Exists pl pr.
-           entailer!.
-        -- inversion H; subst.
-           inversion H5; subst.
-           simpl in *; assumption.
-    + simpl in *.
-      Intros pl_head pr_head.
-      Check (IHb1 z z0 b1 b2 head pl_head pl_head pr_head).
-      sep_apply (IHb1 k' v' l' r' curr pl_head pl pr).
-      sep_apply IHb1.
-
-      destruct l'.
-      *  *)
-
- 
 Theorem hole_rep_fuse_left : forall b k curr_k v l r (curr head pl pr: val),
   well_ordered b ->
   search_path k b (node (curr_k, v) l r) ->
@@ -1128,65 +457,6 @@ Proof.
               simpl in *; lia.
 Admitted.
 
-Lemma no_infinite_node_left {A} : forall (a: A) l r,
-  node a l r <> l.
-Proof.
-  unfold not.
-  intros.
-  induction l.
-  - discriminate.
-  - apply IHl1.
-    inversion H.
-    rewrite H2 at 1.
-    reflexivity.
-Qed.
-
-Lemma no_infinite_node_right {A} : forall (a: A) l r,
-  node a l r <> r.
-Proof.
-  unfold not.
-  intros.
-  induction r.
-  - discriminate.
-  - apply IHr2.
-    inversion H.
-    rewrite H3 at 1.
-    reflexivity.
-Qed.
-
-Fixpoint depth {A} (b: bin_tree A) : nat := 
-  match b with 
-  | leaf => 0
-  | node a l r => S (max (depth l) (depth r))
-  end.
-
-Theorem subtree_depth_monotonic {A} : forall (b1 b2: bin_tree A),
-  is_subtree b1 b2 -> (depth b1 <= depth b2)%nat.
-Proof.
-  intros.
-  dependent induction H; simpl; lia.
-Qed.
-
-Theorem no_subtree_cycle_left {A} : forall (a: A) l r,
-  not (is_subtree (node a l r) l).
-Proof.
-  unfold not.
-  intros.
-  apply subtree_depth_monotonic in H.
-  simpl in H.
-  lia.
-Qed.
-
-Theorem no_subtree_cycle_right {A} : forall (a: A) l r,
-  not (is_subtree (node a l r) r).
-Proof.
-  unfold not.
-  intros.
-  apply subtree_depth_monotonic in H.
-  simpl in H.
-  lia.
-Qed.
-
 Theorem body_search_bst: semax_body Vprog Gprog f_search_bst search_bst_spec.
 Proof.
   start_function.
@@ -1281,46 +551,6 @@ Proof.
         contradiction.
     + apply hole_rep_fuse_right; assumption.
 Qed.
-
-Definition ptr_to_bst_rep b p := EX q, data_at Ews (tptr t_bst) q p * bst_rep b q.
-
-Theorem generalize_ptr_to_node_rep : forall b p q,
-  data_at Ews (tptr t_bst) q p * bst_rep b q |-- ptr_to_bst_rep b p.
-Proof.
-  intros.
-  unfold ptr_to_bst_rep.
-  EExists.
-  entailer!.
-Qed.
-
-(* Definition bst_hole_ptr_rep b p :=
-  match b with
-  | hole => emp
-  | _ => EX q, data_at Ews (tptr t_bst) q p * bst_hole_rep b q
-  end. *)
-Print bst_hole_rep.
-Fixpoint ptr_to_bst_hole_rep b p := 
-  match b with 
-  | hole => emp
-  | node_hole_l (k,v) l r =>
-      EX (q pr: val),
-        data_at Ews (tptr t_bst) q p *
-        malloc_token Ews t_bst q *
-        field_at Ews t_bst [StructField _key] (Vint (Int.repr k)) q *
-        field_at Ews t_bst [StructField _val] (Vint (Int.repr v)) q *
-        field_at Ews t_bst [StructField _right] pr q *
-        ptr_to_bst_hole_rep l (field_address t_bst [StructField _left] q) *
-        bst_rep r pr
-  | node_hole_r (k,v) l r =>
-      EX (q pl: val),
-        data_at Ews (tptr t_bst) q p *
-        malloc_token Ews t_bst q *
-        field_at Ews t_bst [StructField _key] (Vint (Int.repr k)) q *
-        field_at Ews t_bst [StructField _val] (Vint (Int.repr v)) q *
-        field_at Ews t_bst [StructField _left] pl q *
-        bst_rep l pl *
-        ptr_to_bst_hole_rep r (field_address t_bst [StructField _right] q)
-  end.
 
 Theorem body_insert_bst: semax_body Vprog Gprog f_insert_bst insert_bst_spec.
 Proof.
@@ -1746,3 +976,191 @@ Proof.
                 simpl in H6; lia.
   }
 Admitted.
+
+Theorem path_shrink_l : forall k k' v l r b,
+  (* well_ordered (node (k',v) l r) -> *)
+  node (k',v) l r <> b ->
+  k < k' -> search_path k (node (k',v) l r) b -> search_path k l b.
+Proof.
+  (* intros.
+  induction l.
+  - inversion H2; subst.
+    + contradiction.
+    + assumption.
+    + lia.
+  - destruct a.
+    reflect_destruct_Z_compare k z.
+    + inversion H1; subst; try lia.
+      *  *)
+Admitted.
+
+
+Theorem body_pop_min: semax_body Vprog Gprog f_pop_min pop_min_spec.
+Proof.
+  start_function.
+  forward_loop (
+    EX a' l' r' curr_ptr min_z,
+      PROP (
+        min_z = fst (get_min a l r);
+        search_path min_z (node a l r) (node a' l' r');
+        node a' l' r' = node a l r -> curr_ptr = bst_ptr)
+      LOCAL (
+        gvars gv; temp _bst_ptr curr_ptr)
+      SEP (
+        ptr_to_bst_hole_rep (bst_subtract_path min_z (node a l r) (node a' l' r')) bst_ptr;
+        ptr_to_bst_rep (node a' l' r') curr_ptr;
+        mem_mgr gv)
+  ).
+  {
+    entailer!.
+    Exists a l r bst_ptr (fst (get_min a l r)).
+    entailer!.
+    - constructor.
+    - simpl.
+      destruct_pair.
+      Intros pl pr.
+      rewrite Z.compare_refl.
+      unfold ptr_to_bst_rep, ptr_to_bst_hole_rep.
+      expand bst_rep.
+      Exists head pl pr.
+      entailer!.
+  }
+  unfold ptr_to_bst_rep.
+  Intros a' l' r' curr_ptr min_z curr.
+  expand bst_rep.
+  destruct_pair.
+  Intros pl pr.
+  repeat forward.
+  forward_if.
+  {
+    repeat forward.
+    simpl offset_val.
+    assert_PROP (l' <> leaf) by (entailer!; find_contradiction).
+    destruct l' as [|l'a l'l l'r]; [contradiction|].
+    entailer!.
+    simplify_assumps; subst.
+    Exists l'a l'l l'r (field_address t_bst [StructField _left] curr) (fst (get_min a l r)).
+    entailer!.
+    - split.
+      + eapply path_step_down_l; [eassumption|].
+        apply get_min_is_min in H0.
+        admit.
+      + intros. inversion H14; subst.
+        exfalso; eapply no_subtree_cycle_left.
+        eapply search_path_is_subtree.
+        eassumption.
+    - 
+      sep_apply generalize_node_rep.
+      simpl bst_subtract_path.
+      repeat destruct_pair.
+      rewrite Zaux.Zcompare_Lt.
+      rewrite Zaux.Zcompare_Lt.
+      + clear - H0 H2 H3.   
+        simpl.
+        Intros pl pr pl0 pr0 q pr1.
+        Exists pl0 pr0.
+        cancel.
+        unfold ptr_to_bst_rep.
+        Exists pl.
+        expand bst_rep.
+        Exists q pr1.
+        cancel.
+        unfold_data_at (data_at _ _ _ curr).
+        cancel.
+
+        clear H3.   
+        revert z3 z4 r H0 H2 pl0.
+        induction l; intros.
+        * simpl in H2. inversion H2; lia.
+        *
+          simpl in *.
+          destruct_pair. 
+          rewrite Zaux.Zcompare_Lt.
+          rewrite Zaux.Zcompare_Lt.
+          {
+            simpl.
+            Intros q0 pr2. Exists q0 pr2.
+            sep_apply (IHl1 z5 z6 l2).
+            - inversion H0; assumption.
+            - eapply path_shrink_l; [| |eassumption].
+              + injection; intros; subst. 
+          }
+          
+  }
+  repeat forward.
+  simplify_assumps; subst.
+  simpl bst_subtract_path.
+  destruct_pair.
+  rewrite Zaux.Zcompare_Lt. (* Since search_path puts z towards the min *)
+  simpl ptr_to_bst_hole_rep.
+  Intros q pr0. (* generalize pr0? *)
+  Exists curr q.
+  (* EExists. *)
+  expand bst_rep.
+  destruct (get_min (z1, z2) l r) eqn:H_min.
+  (* Exists nullval. *)
+  (* EExists. *)
+  (* entailer!. *)
+  clear - H0 H2 H3 H_min.
+  revert pr0.
+  induction l; intros.
+  - simpl in *.
+    inversion H_min; subst.
+    inversion H2; subst; try lia.
+    simplify_assumps; subst.
+Admitted.
+
+Theorem body_delete_bst: semax_body Vprog Gprog f_delete_bst delete_bst_spec.
+Proof.
+  start_function.
+  forward.
+  forward_if.
+  {
+    forward.
+    EExists.
+    simplify_assumps; subst.
+    entailer!.
+  }
+  assert_PROP (b <> leaf) by (expand bst_rep; entailer!; find_contradiction). 
+  destruct b as [|[parent_k v] l r]; [contradiction|].
+  expand bst_rep.
+  Intros pl pr.
+  repeat (forward + forward_if).
+  {
+    assert_PROP (r <> leaf) by (expand bst_rep; entailer!; find_contradiction). 
+    destruct r as [|ra rl rr]; [contradiction|].
+    assert_PROP (field_compatible t_bst [StructField _right] parent) by entailer!.
+    forward_call(
+      field_address t_bst [StructField _right] parent,
+      pr, ra, rl, rr, gv).
+    - unfold_data_at (data_at _ _ _ parent).
+      entailer!.
+    - split.
+      + inversion H0; assumption.
+      + inversion H1; assumption.
+    - Intros vret.
+      expand bst_rep.
+      destruct (get_min ra rl rr) eqn:H_min.
+      Intros pl0 pr0.
+      repeat forward.
+      forward_call(t_bst, fst (fst vret), gv).
+      { entailer!.
+        apply field_compatible_nullval1 in H15.
+        destruct (eq_dec (fst (fst vret)) nullval); [contradiction|].
+        entailer!. }
+      Exists parent.
+      entailer!.
+      enough (k = parent_k).
+      subst.
+      simpl.
+      rewrite Z.compare_refl.
+      assert_PROP (l <> leaf) by (expand bst_rep; entailer!; find_contradiction). 
+      destruct l as [|la ll lr]; [contradiction|].
+      expand bst_rep.
+      destruct la.
+      rewrite H_min.
+      Exists pl (snd (fst vret)).
+      Intros pl0 pr1; Exists pl0 pr1.
+      unfold_data_at (data_at _ _ _ parent).
+      entailer!.
+  }
