bst_holes.v
@@ -1,0 +1,155 @@
+Require Import VST.floyd.proofauto.
+(* Require Import Coq.Program.Equality. *)
+
+Require Import my_tactics.
+Require Import bst_spec.
+
+(* bin_tree with *exactly* one hole *)
+Inductive bin_tree_hole (A: Type) : Type :=
+  | hole : bin_tree_hole A
+  | node_hole_l : A -> bin_tree_hole A -> bin_tree A -> bin_tree_hole A
+  | node_hole_r : A -> bin_tree A -> bin_tree_hole A -> bin_tree_hole A.
+Arguments bin_tree_hole _%type_scope.
+Arguments hole {A}%type_scope.
+Arguments node_hole_l {A}%type_scope.
+Arguments node_hole_r {A}%type_scope.
+
+Fixpoint fill_hole {A} (outer: bin_tree_hole A) (inner: bin_tree A) : bin_tree A :=
+  match outer with 
+  | hole => inner
+  | node_hole_l a l r => node a (fill_hole l inner) r
+  | node_hole_r a l r => node a l (fill_hole r inner)
+  end.
+
+Fixpoint extend_hole {A} (outer inner: bin_tree_hole A) : bin_tree_hole A :=
+  match outer with 
+  | hole => inner
+  | node_hole_l a l r => node_hole_l a (extend_hole l inner) r
+  | node_hole_r a l r => node_hole_r a l (extend_hole r inner)
+  end.
+
+Definition bst_hole A := bin_tree_hole (Z * A).
+
+(* This acts as a complement to search - where search returns the subtree, this returns the original tree,
+   but with a hole where the subtree used to be. *)
+Fixpoint search_make_hole {A} (k: Z) (b: bst A) : bst_hole A := 
+  match b with 
+  | leaf => hole
+  | node (k', v) l r => 
+      match k ?= k' with 
+      | Eq => hole
+      | Lt => node_hole_l (k', v) (search_make_hole k l) r
+      | Gt => node_hole_r (k', v) l (search_make_hole k r)
+      end 
+  end.
+
+Theorem fill_search_hole {A} : forall k (b: bst A),
+  fill_hole (search_make_hole k b) (search k b) = b.
+Proof.
+  intros k b.
+  induction b.
+  - reflexivity.
+  - simpl.
+    destruct_pair.
+    find_Z_compare_destruct; simpl.
+    + reflexivity.
+    + f_equal. assumption.
+    + f_equal. assumption.
+Qed.
+
+(* This does search and search_make_hole together *)
+Fixpoint split_bst_at {A} (k: Z) (b: bst A) : bst_hole A * bst A :=
+  match b with 
+  | leaf => (hole, leaf)
+  | node (k', v) l r =>
+      match k ?= k' with 
+      | Eq => (hole, b)
+      | Lt => let (outer, inner) := split_bst_at k l 
+              in (node_hole_l (k', v) outer r, inner)
+      | Gt => let (outer, inner) := split_bst_at k r 
+              in (node_hole_r (k', v) l outer, inner)
+      end 
+  end.
+
+(* Intended for when `search_path k outer inner` *)
+Definition bst_subtract_path k (outer inner: bst Z) : bst_hole Z :=
+  match inner with 
+  | leaf => search_make_hole k outer
+  | node (k',v) l r => search_make_hole k' outer 
+  end.
+
+Lemma bst_subtract_path_b_b : forall k b, bst_subtract_path k b b = hole.
+Proof.
+  intros.
+  destruct b.
+  - reflexivity.
+  - simpl.
+    destruct_pair.
+    rewrite Z.compare_refl.
+    reflexivity.
+Qed.
+
+Theorem fill_hole_bst_subtract_path: forall k b sub,
+  well_ordered b ->
+  search_path k b sub ->
+  fill_hole (bst_subtract_path k b sub) sub = b.
+Proof.
+  intros k b sub H_wo H_path.
+  induction H_path.
+  - destruct b.
+    + reflexivity.
+    + simpl.
+      destruct_pair.
+      rewrite Z.compare_refl.
+      reflexivity.
+  - inversion H_wo; subst.
+    simplify_assumps.
+    destruct b.
+    + simpl.
+      rewrite Zaux.Zcompare_Lt by assumption.
+      simpl.
+      f_equal.
+      simpl in *.
+      assumption.
+    + simpl.
+      destruct_pair.
+      simpl in *.
+      apply search_path_is_subtree in H_path.
+      find_Z_compare_destruct.
+      * eapply subtree_forall in H_path; [|eassumption].
+        inversion H_path; subst.
+        simpl in *.
+        lia.
+      * simpl.
+        f_equal.
+        assumption.
+      * eapply subtree_forall in H_path; [|eapply H4].
+        inversion H_path; subst.
+        simpl in *.
+        lia.
+  - inversion H_wo; subst.
+    simplify_assumps.
+    destruct b.
+    + simpl.
+      rewrite Zaux.Zcompare_Gt by lia.
+      simpl.
+      f_equal.
+      simpl in *.
+      assumption.
+    + simpl.
+      destruct_pair.
+      simpl in *.
+      apply search_path_is_subtree in H_path.
+      find_Z_compare_destruct.
+      * eapply subtree_forall in H_path; [|eassumption].
+        inversion H_path; subst.
+        simpl in *.
+        lia.
+      * eapply subtree_forall in H_path; [|eapply H5].
+        inversion H_path; subst.
+        simpl in *.
+        lia.
+      * simpl.
+        f_equal.
+        assumption.
+Qed.
