bst_spec.v
@@ -1,0 +1,572 @@
+Require Import VST.floyd.proofauto.
+Require Import Coq.Program.Equality.
+
+Require Import my_tactics.
+
+Inductive bin_tree (A: Type) : Type := 
+  | leaf : bin_tree A
+  | node : A -> bin_tree A -> bin_tree A -> bin_tree A.
+Arguments bin_tree _%type_scope.
+Arguments leaf {A}%type_scope.
+Arguments node {A}%type_scope.
+
+Inductive bin_tree_forall {A} : bin_tree A -> (A -> Prop) -> Prop :=
+  | bin_tree_forall_leaf : forall p, bin_tree_forall leaf p 
+  | bin_tree_forall_node : forall (p: A -> Prop) a l r,
+      p a -> bin_tree_forall l p -> bin_tree_forall r p -> bin_tree_forall (node a l r) p.
+
+Theorem bin_tree_forall_strengthen {A} : forall (p q: A -> Prop) b,
+  (forall x, p x -> q x) -> bin_tree_forall b p -> bin_tree_forall b q.
+Proof.
+  intros.
+  dependent induction H0; subst; constructor; simplify_assumps.
+  - apply H. assumption.
+  - assumption.
+  - assumption.
+Qed.
+
+Inductive well_ordered {A} : bin_tree (Z * A) -> Prop :=
+  | well_ordered_leaf : well_ordered leaf 
+  | well_ordered_node : forall k v l r,
+      bin_tree_forall l (fun n => fst n < k) -> 
+      bin_tree_forall r (fun n => fst n > k) -> 
+      well_ordered l ->
+      well_ordered r ->
+      well_ordered (node (k, v) l r).
+
+Definition bst A := bin_tree (Z * A).
+
+(* Subtrees *)
+
+Inductive is_subtree {A} : bin_tree A -> bin_tree A -> Prop :=
+  | is_subtree_refl  : forall b, is_subtree b b 
+  | is_subtree_left  : forall b n l r, is_subtree b l -> is_subtree b (node n l r)
+  | is_subtree_right : forall b n l r, is_subtree b r -> is_subtree b (node n l r).
+
+(* Definition proper_subtree {A} (b1 b2: bin_tree A) := b1 <> b2 /\ is_subtree b1 b2. *)
+
+Lemma is_subtree_leaf : forall {A} (b: bin_tree A), is_subtree leaf b.
+Proof.
+  intros A b.
+  induction b; constructor; assumption.
+Qed.
+
+Theorem subtree_forall : forall {A} sub b (p: A -> Prop),
+  is_subtree sub b -> bin_tree_forall b p -> bin_tree_forall sub p.
+Proof.
+  intros.
+  induction H;
+  try (apply IHis_subtree; inversion H0);
+  assumption.
+Qed.
+
+Theorem subtree_well_ordered : forall {A} (b sub: bst A),
+  is_subtree sub b -> well_ordered b -> well_ordered sub.
+Proof.
+  intros.
+  induction b.
+  - destruct sub.
+    + constructor.
+    + inversion H.
+  - inversion H; subst.
+    + assumption.
+    + inversion H0; apply IHb1; assumption.
+    + inversion H0; apply IHb2; assumption.
+Qed.
+
+Theorem is_subtree_up_left {A}: forall (a: A) l r b,
+  is_subtree (node a l r) b -> is_subtree l b.
+Proof.
+  intros.
+  dependent induction H.
+  - apply is_subtree_left. constructor.
+  - apply is_subtree_left.
+    eapply IHis_subtree.
+    reflexivity.
+  - apply is_subtree_right.
+    eapply IHis_subtree.
+    reflexivity.
+Qed.
+
+Theorem is_subtree_up_right {A}: forall (a: A) l r b,
+  is_subtree (node a l r) b -> is_subtree r b.
+Proof.
+  intros.
+  dependent induction H.
+  - apply is_subtree_right. constructor.
+  - apply is_subtree_left.
+    eapply IHis_subtree.
+    reflexivity.
+  - apply is_subtree_right.
+    eapply IHis_subtree.
+    reflexivity.
+Qed.
+
+Lemma no_infinite_node_left {A} : forall (a: A) l r,
+  node a l r <> l.
+Proof.
+  unfold not.
+  intros.
+  induction l.
+  - discriminate.
+  - apply IHl1.
+    inversion H.
+    rewrite H2 at 1.
+    reflexivity.
+Qed.
+
+Lemma no_infinite_node_right {A} : forall (a: A) l r,
+  node a l r <> r.
+Proof.
+  unfold not.
+  intros.
+  induction r.
+  - discriminate.
+  - apply IHr2.
+    inversion H.
+    rewrite H3 at 1.
+    reflexivity.
+Qed.
+
+Fixpoint depth {A} (b: bin_tree A) : nat := 
+  match b with 
+  | leaf => 0
+  | node a l r => S (max (depth l) (depth r))
+  end.
+
+Theorem subtree_depth_monotonic {A} : forall (b1 b2: bin_tree A),
+  is_subtree b1 b2 -> (depth b1 <= depth b2)%nat.
+Proof.
+  intros.
+  dependent induction H; simpl; lia.
+Qed.
+
+Theorem no_subtree_cycle_left {A} : forall (a: A) l r,
+  not (is_subtree (node a l r) l).
+Proof.
+  unfold not.
+  intros.
+  apply subtree_depth_monotonic in H.
+  simpl in H.
+  lia.
+Qed.
+
+Theorem no_subtree_cycle_right {A} : forall (a: A) l r,
+  not (is_subtree (node a l r) r).
+Proof.
+  unfold not.
+  intros.
+  apply subtree_depth_monotonic in H.
+  simpl in H.
+  lia.
+Qed.
+
+Lemma wo_node_eq {A} : forall k (v1 v2: A) l1 l2 r1 r2,
+  well_ordered (node (k,v1) l1 r1) ->
+  is_subtree (node (k,v2) l2 r2) (node (k,v1) l1 r1) ->
+  node (k,v1) l1 r1 = node (k,v2) l2 r2.
+Proof.
+  intros.
+  inversion H0; subst.
+  - reflexivity. 
+  - inversion H; subst. 
+    eapply subtree_forall in H3; [|eassumption].
+    inversion H3; subst.
+    simpl in H5. lia.
+  - inversion H; subst. 
+    eapply subtree_forall in H3; [|eassumption].
+    inversion H3; subst.
+    simpl in H5. lia.
+Qed.
+
+Lemma wo_subtree_left {A} : forall k1 k2 (v1 v2: A) l1 l2 r1 r2,
+  well_ordered (node (k1,v1) l1 r1) ->
+  is_subtree (node (k2,v2) l2 r2) (node (k1,v1) l1 r1) ->
+  k2 < k1 ->
+  is_subtree (node (k2,v2) l2 r2) l1.
+Proof.
+  intros.
+  inversion H0; subst.
+  - lia.
+  - assumption.
+  - inversion H; subst.
+    eapply subtree_forall in H4; [|eassumption].
+    inversion H4; subst.
+    simpl in H6. lia.
+Qed.
+
+Lemma wo_subtree_right {A} : forall k1 k2 (v1 v2: A) l1 l2 r1 r2,
+  well_ordered (node (k1,v1) l1 r1) ->
+  is_subtree (node (k2,v2) l2 r2) (node (k1,v1) l1 r1) ->
+  k2 > k1 ->
+  is_subtree (node (k2,v2) l2 r2) r1.
+Proof.
+  intros.
+  inversion H0; subst.
+  - lia.
+  - inversion H; subst.
+    eapply subtree_forall in H4; [|eassumption].
+    inversion H4; subst.
+    simpl in H6. lia.
+  - assumption.
+Qed.
+
+(* Search *)
+
+Fixpoint search {A} (k: Z) (b: bst A) : bst A := 
+  match b with 
+  | leaf => leaf
+  | node (k', v) l r => 
+      match k ?= k' with 
+      | Eq => b
+      | Lt => search k l
+      | Gt => search k r
+      end 
+  end.
+
+Theorem search_spec {A} : forall (b: bst A) k v l r,
+  well_ordered b ->
+  is_subtree (node (k,v) l r) b ->
+  search k b = node (k,v) l r.
+Proof.
+  intros.
+  induction b.
+  - inversion H0.
+  - inversion H; subst.
+    simplify_assumps.
+    simpl.
+    find_Z_compare_destruct.
+    + eapply wo_node_eq; assumption.
+    + apply IHb1.
+      eapply wo_subtree_left; eassumption.
+    + apply IHb2.
+      eapply wo_subtree_right; eassumption.
+Qed.
+
+Theorem search_is_subtree : forall {A} k (b sub: bst A),
+  search k b = sub -> is_subtree sub b.
+Proof.
+  intros A k b sub.
+  induction b; try destruct_pair; simpl; intro H.
+  - subst. constructor.
+  - find_Z_compare_destruct.
+    + constructor.
+    + apply is_subtree_left.
+      apply IHb1.
+      assumption.
+    + apply is_subtree_right.
+      apply IHb2.
+      assumption.
+Qed.
+
+Lemma search_well_ordered : forall {A} k (b sub: bst A),
+  search k b = sub -> well_ordered b -> well_ordered sub.
+Proof.
+  intros.
+  eapply subtree_well_ordered.
+  eapply search_is_subtree.
+  eassumption.
+  assumption.
+Qed.
+
+(* Insert *)
+
+Fixpoint insert {A} (k: Z) (v: A) (b: bst A) : bst A :=
+  match b with 
+  | leaf => node (k, v) leaf leaf
+  | node (k', v') l r => 
+      match k ?= k' with 
+      | Eq => node (k', v) l r 
+      | Lt => node (k', v') (insert k v l) r 
+      | Gt => node (k', v') l (insert k v r)
+      end 
+  end.
+
+Lemma insert_forall {A} : forall (p: (Z * A) -> Prop) k v bst,
+  p (k, v) -> bin_tree_forall bst p -> bin_tree_forall (insert k v bst) p.
+Proof.
+  intros p k v b H.
+  induction b; intro H0; simpl.
+  - constructor; assumption.
+  - destruct_pair. find_Z_compare_destruct;
+    inversion H0; subst; constructor; 
+    try (apply IHb1 + apply IHb2); 
+    assumption.
+Qed.
+
+Theorem insert_well_ordered {A}: forall (b: bst A) k v, 
+  well_ordered b -> well_ordered (insert k v b).
+Proof.
+  intro b; induction b; intros k v H; simpl.
+  - repeat constructor.
+  - inversion H; subst.
+    find_Z_compare_destruct;
+    constructor; try (apply insert_forall + apply IHb1 + apply IHb2); assumption.
+Qed.
+
+Theorem search_insert {A}: forall k v (b: bst A),
+  exists l r, search k (insert k v b) = node (k, v) l r.
+Proof.
+  intros k v b.
+  induction b.
+  - simpl.
+    rewrite Z.compare_refl.
+    unify_goal.
+  - simpl. destruct_pair.
+    find_Z_compare_destruct;
+    simpl; rewrite Heqc; assumption + unify_goal.
+Qed.
+
+(* Delete *)
+
+Fixpoint get_min {A} (a: Z * A) (l r: bst A) : Z * A :=
+  match l with
+  | leaf => a
+  | node a' l' r' => get_min a' l' r'
+  end.
+
+Fixpoint rm_min {A} (a: Z * A) (l r: bst A) : bst A :=
+  match l with
+  | leaf => r
+  | node a' l' r' => node a (rm_min a' l' r') r
+  end.
+
+Lemma get_min_forall {A} : forall (p: (Z * A) -> Prop) a l r,
+  bin_tree_forall (node a l r) p -> p (get_min a l r).
+Proof.
+  intros p a l; revert p a.
+  induction l; intros; simpl.
+  - inversion H; assumption.
+  - apply IHl1.
+    inversion H; assumption.
+Qed.
+
+Lemma rm_min_forall {A} : forall (p: (Z * A) -> Prop) a l r,
+  bin_tree_forall (node a l r) p -> bin_tree_forall (rm_min a l r) p.
+Proof.
+  intros p a l; revert p a.
+  induction l; intros; simpl.
+  - inversion H; assumption.
+  - constructor.
+    + inversion H; assumption.
+    + apply IHl1. inversion H; assumption.
+    + inversion H; assumption.
+Qed.
+
+Lemma get_min_is_min {A} : forall (a: Z * A) l r,
+  well_ordered (node a l r) ->
+  bin_tree_forall (rm_min a l r) (fun n => fst n > fst (get_min a l r)).
+Proof.
+  intros a l; revert a.
+  induction l; intros; simpl.
+  - inversion H; assumption.
+  - constructor.
+    + inversion H; subst.
+      apply get_min_forall in H3.
+      simpl. lia.
+    + apply IHl1. inversion H; assumption.
+    + inversion H; subst.
+      eapply bin_tree_forall_strengthen; [|eassumption].
+      intros [x].
+      simpl.
+      enough (k > fst (get_min a l1 l2)); [lia|].
+      apply get_min_forall in H3.
+      lia.
+Qed.
+
+Lemma get_min_is_min_2 {A} : forall (a: Z * A) l r,
+  well_ordered (node a l r) ->
+  bin_tree_forall (node a l r) (fun n => fst n >= fst (get_min a l r)).
+Proof.
+  intros a l; revert a.
+  induction l; intros; simpl.
+  - inversion H; subst.
+    constructor.
+    + lia.
+    + constructor.
+    + simpl.
+      eapply bin_tree_forall_strengthen; [|eassumption]. 
+      intros [x].
+      lia.
+  - inversion H; subst.
+    constructor.
+    + specialize (IHl1 a l2 H5).
+      inversion IHl1; subst.
+      simpl.
+      inversion H3; subst.
+      lia.
+    + apply IHl1.
+      assumption.
+    + eapply bin_tree_forall_strengthen; [|eassumption]. 
+      intros [x].
+      simpl.
+      enough (k > fst (get_min a l1 l2)); [lia|].
+      apply get_min_forall in H3.
+      lia.
+Qed.
+
+Theorem rm_min_well_ordered {A} : forall (a: Z * A) l r,
+  well_ordered (node a l r) -> well_ordered (rm_min a l r).
+Proof.
+  intros a l; revert a.
+  induction l; intros; simpl.
+  - inversion H; assumption.
+  - destruct a0; constructor.
+    + apply rm_min_forall. inversion H; assumption.
+    + inversion H; assumption.
+    + apply IHl1. inversion H; assumption.
+    + inversion H; assumption.
+Qed.
+
+Fixpoint delete {A} (k: Z) (b: bst A) : bst A := 
+  match b with 
+  | leaf => leaf
+  | node (k', v) l r => 
+      match k ?= k' with 
+      | Eq => match l with
+          | leaf => r
+          | _ => match r with 
+              | leaf => leaf
+              | node ra rl rr => node (get_min ra rl rr) l (rm_min ra rl rr)
+              end
+          end
+      | Lt => delete k l
+      | Gt => delete k r
+      end 
+  end.
+
+Lemma delete_forall {A} : forall (p: (Z * A) -> Prop) k bst,
+  bin_tree_forall bst p -> bin_tree_forall (delete k bst) p.
+Proof.
+  intros p k b.
+  induction b as [|[k' v] l IH1 r IH2]; intro H; simpl; [assumption|].
+  find_Z_compare_destruct.
+  - destruct l, r; try (inversion H; assumption).
+    constructor.
+    + apply get_min_forall.
+      inversion H; assumption.
+    + inversion H; assumption.
+    + apply rm_min_forall.
+      inversion H; assumption.
+  - apply IH1. inversion H; assumption.
+  - apply IH2. inversion H; assumption.
+Qed.
+
+Theorem delete_well_ordered {A}: forall (b: bst A) k, 
+  well_ordered b -> well_ordered (delete k b).
+Proof.
+  intros b; induction b as [|[k' v] l IH1 r IH2]; intros k H; simpl; [constructor|].
+  find_Z_compare_destruct.
+  - destruct l, r; try (inversion H; assumption).
+    destruct (get_min p0 r1 r2) eqn:H_min.
+    constructor.
+    + inversion H; subst.
+      eapply bin_tree_forall_strengthen; [|eassumption].
+      intros [x].
+      simpl.
+      enough (k' < z); [lia|].
+      apply get_min_forall in H5.
+      rewrite H_min in H5; simpl in H5.
+      lia.
+    + replace z with (fst (get_min p0 r1 r2)) by (rewrite H_min; reflexivity).
+      apply get_min_is_min.
+      inversion H; assumption.
+    + inversion H; assumption.
+    + apply rm_min_well_ordered.
+      inversion H; assumption.
+  - apply IH1. inversion H; assumption.
+  - apply IH2. inversion H; assumption.
+Qed.
+
+(* search_path: This describes a point in a key-search traversal, commonly used to express 
+   loop invariants *)
+
+(* The direction of transitivity here is nice for induction, but doesn't correspond 
+   to the intuitive direction in which a path grows. *)
+Inductive search_path : Z -> bst Z -> bst Z -> Prop := 
+  | path_refl : forall k b, search_path k b b
+  | path_step_l : forall k k' v l r b,
+      search_path k l b -> k < k' -> search_path k (node (k',v) l r) b
+  | path_step_r : forall k k' v l r b,
+      search_path k r b -> k > k' -> search_path k (node (k',v) l r) b.
+
+(* This is the direction a path will actually grow in *)
+Lemma path_step_down_l : forall k head k' v l r,
+  search_path k head (node (k',v) l r) -> k < k' -> search_path k head l.
+Proof.
+  intros. dependent induction H.
+  - apply path_step_l.
+    + constructor. 
+    + assumption.
+  - apply path_step_l.
+    + eapply IHsearch_path; trivial.
+    + assumption. 
+  - apply path_step_r.
+    + eapply IHsearch_path; trivial.
+    + assumption.
+Qed.
+
+Lemma path_step_down_r : forall k head k' v l r,
+  search_path k head (node (k',v) l r) -> k > k' -> search_path k head r.
+Proof.
+  intros. dependent induction H.
+  - apply path_step_r.
+    + constructor. 
+    + assumption.
+  - apply path_step_l.
+    + eapply IHsearch_path; trivial.
+    + assumption. 
+  - apply path_step_r.
+    + eapply IHsearch_path; trivial.
+    + assumption.
+Qed.
+
+Theorem search_path_fail : forall k b, search_path k b leaf -> search k b = leaf.
+Proof.
+  intros. dependent induction H.
+  - reflexivity.
+  - simpl.
+    rewrite Zaux.Zcompare_Lt by assumption.
+    apply IHsearch_path.
+    reflexivity.
+  - simpl.
+    rewrite Zaux.Zcompare_Gt by lia.
+    apply IHsearch_path.
+    reflexivity.
+Qed.
+
+Theorem search_path_success: forall k b v l r,
+  search_path k b (node (k,v) l r) -> search k b = (node (k,v) l r).
+Proof.
+  intros. dependent induction H.
+  - simpl.
+    rewrite Z.compare_refl.
+    reflexivity.
+  - simpl.
+    rewrite Zaux.Zcompare_Lt by assumption. 
+    apply IHsearch_path.
+    reflexivity.
+  - simpl.
+    rewrite Zaux.Zcompare_Gt by lia.
+    apply IHsearch_path.
+    reflexivity.
+Qed.
+
+Lemma search_path_constant : forall k b1 b2,
+  search_path k b1 b2 -> search k b1 = search k b2.
+Proof.
+  intros k b1 b2 H.
+  dependent induction H; simpl.
+  - reflexivity.
+  - rewrite Zaux.Zcompare_Lt; assumption.
+  - rewrite Zaux.Zcompare_Gt by lia. assumption.
+Qed.
+
+Theorem search_path_is_subtree: forall k b sub, search_path k b sub -> is_subtree sub b.
+Proof.
+  intros.
+  induction H.
+  - constructor.
+  - apply is_subtree_left. assumption.
+  - apply is_subtree_right. assumption.
+Qed.
